Verifichiamo che $\forall m,n \in \mathbb Z$ si ha che $$ \underbrace m _{\in A} + \underbrace n _{\in A} = \underbrace{m+n}_{\in A} \qquad \underbrace m _{\in A} \cdot \underbrace n _{\in A} = \underbrace{m\cdot n}_{\in A}$$

**Per la Somma**:
$$ \begin{align*}
\underbrace m _{\in A} + \underbrace n _{\in A} &= (\underbrace{1+1+\;...+1}_{m \text{ volte}}) + (\underbrace{1+1+\; ...+1}_{n \text{ volte}}) = \underbrace{1+1+\; ...+1}_{m+n\text{ volte}} = \underbrace{m+n}_{\in A}\end{align*}$$
**Per il Prodotto**:
$$ \begin{align*}
\underbrace m _{\in A} \cdot \underbrace n _{\in A} &= (\underbrace{1+1+\;...+1}_{m \text{ volte}}) \cdot (\underbrace{1+1+\; ...+1}_{n \text{ volte}}) = \underbrace{(\underbrace{1+1+\; ...+1}_{n \text{ volte}})+...+(\underbrace{1+1+\; ...+1}_{n \text{ volte}})}_{m \text{ volte}} = \underbrace{1+1+\;...+1}_{m \cdot n\text{ volte}}= \underbrace{m\cdot n}_{\in A}
\end{align*}$$