Sia $\overrightarrow f(x_1,x_2,x_3) = (x_1+x_3, x_2^2, x_3x_2^4)$
Allora possiamo calcolare le derivate parziali come:
$$\frac{∂\overrightarrow f}{∂x_1} = \left(\frac{∂}{∂x_1}(x_1+x_3),\frac{∂}{∂x_1}(x_2^2),\frac{∂}{∂x_1}(x_3x_2^4) \right) = (1,0,0)$$
$$\frac{∂\overrightarrow f}{∂x_2} = \left(\frac{∂}{∂x_2}(x_1+x_3),\frac{∂}{∂x_2}(x_2^2),\frac{∂}{∂x_2} (x_3x_2^4)\right) = (0, 2x_2,4_x3x_2^3)$$
$$\frac{∂\overrightarrow f}{∂x_3} = \left(\frac{∂}{∂x_3}(x_1+x_3),\frac{∂}{∂x_3}(x_2^2),\frac{∂}{∂x_3}(x_3x_2^4) \right) = (1,0,x_2^4)$$

*Le derivate parziali di un vettore sono tre vettori*